src/ConcurrentCache.v
@@ -1,0 +1,110 @@
+Require Import CoopConcur.
+Require Import CoopConcurAuto.
+Require Import Protocols.
+Require Import Locking.
+Require Import Star.
+Import List.ListNotations.
+Import Hlist.HlistNotations.
+
+Require Import MemCache.
+
+Section ConcurrentCache.
+
+  Variable Sigma:State.
+
+  Definition CacheSigma := defState [Flags; Cache] [Locks addr; Cache; DISK].
+
+  Variable cacheProj : StateProj Sigma CacheSigma.
+
+  (* memory variables *)
+
+  Definition mLocks := ltac:(hget 0 (memVars cacheProj)).
+  Definition mCache := ltac:(hget 1 (memVars cacheProj)).
+
+  (* abstraction ("virtual") variables *)
+
+  Definition vLocks := ltac:(hget 0 (abstractionVars cacheProj)).
+  Definition vCache := ltac:(hget 1 (abstractionVars cacheProj)).
+  Definition vDisk := ltac:(hget 2 (abstractionVars cacheProj)).
+
+  Definition cacheR (tid:TID) : Relation Sigma :=
+    fun s s' =>
+      let ld := get vDisk s in
+      let ld' := get vDisk s' in
+      let locks := get vLocks s in
+      let locks' := get vLocks s' in
+      same_domain ld ld' /\
+      (* lock protects virtual disk *)
+      (forall a, locks a = Owned tid ->
+            ld' a = ld a) /\
+      lock_protocol tid locks locks'.
+
+  Definition addr_lock (l:Flags) (a:addr) :=
+    get_lock l #a.
+
+  Definition cacheI : Invariant Sigma :=
+    fun d m s =>
+      get mCache m = get vCache s /\
+      locks_rep (addr_lock (get mLocks m)) (get vLocks s) /\
+      cache_rep d (get vCache s) (get vDisk s).
+
+  Variable delta:Protocol Sigma.
+
+  Hint Resolve same_domain_refl.
+  Hint Resolve lock_protocol_refl.
+
+  Theorem cacheR_trans_closed : forall tid s s',
+      star (cacheR tid) s s' ->
+      cacheR tid s s'.
+  Proof.
+    intros.
+    apply trans_closed; auto; intuition.
+    unfold cacheR; intuition.
+    admit.
+  Admitted.
+
+  Definition CacheProtocol : Protocol Sigma :=
+    defProtocol cacheI cacheR cacheR_trans_closed.
+
+  Hypothesis cacheProtocolDerive : SubProtocol delta CacheProtocol.
+  Hypothesis cacheProtocolRespected : SubProtocolUnder
+                                        (privateVars [( mLocks; mCache )] [( vLocks; vCache )])
+                                        CacheProtocol delta.
+
+  Definition cache_maybe_read {T} a rx : prog Sigma T :=
+    c <- Get mCache;
+      rx (cache_val c a).
+
+  Definition cache_write {T} a v rx : prog Sigma T :=
+    c <- Get mCache;
+      let c' := cache_add c a (Dirty v) in
+      Assgn mCache c';;
+            rx tt.
+
+  (* TODO: add ghost updates for reader state *)
+  Definition AsyncRead {T} a rx : prog Sigma T :=
+    StartRead a;;
+              Yield a;;
+              v <- FinishRead a;
+      rx v.
+
+  Definition lock {T} (a: addr) rx : prog Sigma T :=
+    tid <- GetTID;
+      wait_for mLocks (is_open #a) a;;
+               l <- Get mLocks;
+      Assgn mLocks (set_locked l #a);;
+            GhostUpdate
+            (fun s =>
+               let l := get vLocks s in
+               let l' := upd_lock l a (Owned tid) in
+               set vLocks l' s);;
+            rx tt.
+
+  Definition cache_fill {T} a rx : prog Sigma T :=
+    v <- AsyncRead a;
+      c <- Get mCache;
+      let c' := cache_add c a (Clean v) in
+      Assgn mCache c';;
+            rx tt.
+
+End ConcurrentCache.
