src/DiskReaders.v
@@ -1,0 +1,20 @@
+Require Import CoopConcur.
+
+Definition Disk:Type := @mem addr (@weq addrlen) (const valu).
+Definition hide_readers (d:DISK) : Disk :=
+  fun a => match d a with
+        | Some (v, _) => Some v
+        | None => None
+        end.
+
+Definition add_reader (d:DISK) a tid :=
+  match d a with
+  | Some (v, _) => upd d a (v, Some tid)
+  | _ => d
+  end.
+
+Definition remove_reader (d:DISK) a :=
+  match d a with
+  | Some (v, _) => upd d a (v, None)
+  | _ => d
+  end.
